theories/examples/disjoint_regions_tactics.v
@@ -1,4 +1,4 @@
-From iris.proofmode Require Import tactics.
+From iris.proofmode Require Import proofmode.
 From stdpp Require Import sets list.
 From cap_machine Require Import addr_reg region.
 
