theories/ftlr/LoadU.v
@@ -1,5 +1,5 @@
 From stdpp Require Import base.
-From iris.proofmode Require Import tactics.
+From iris.proofmode Require Import proofmode.
 From iris.program_logic Require Import weakestpre adequacy lifting.
 From cap_machine Require Export logrel.
 From cap_machine Require Import ftlr_base.
@@ -9,7 +9,7 @@ Import uPred.
 
 Section fundamental.
   Context {Σ:gFunctors} {memg:memG Σ} {regg:regG Σ}
-          {stsg : STSG Addr region_type Σ} {heapg : heapG Σ}
+          {stsg : STSG Addr region_type Σ} {heapg : heapGS Σ}
           {nainv: logrel_na_invs Σ}
           `{MP: MachineParameters}.
 
