theories/rules/rules_Jnz.v
@@ -1,7 +1,7 @@
 From cap_machine Require Import rules_base.
 From iris.base_logic Require Export invariants gen_heap.
 From iris.program_logic Require Export weakestpre ectx_lifting.
-From iris.proofmode Require Import tactics.
+From iris.proofmode Require Import proofmode.
 From iris.algebra Require Import frac.
 
 Section cap_lang_rules.
@@ -49,14 +49,14 @@ Section cap_lang_rules.
         [∗ map] k↦y ∈ regs', k ↦ᵣ y }}}.
   Proof.
     iIntros (Hinstr Hvpc HPC Dregs φ) "(>Hpc_a & >Hmap) Hφ".
-    iApply wp_lift_atomic_head_step_no_fork; auto.
+    iApply wp_lift_atomic_base_step_no_fork; auto.
     iIntros (σ1 l1 l2 n) "Hσ1 /=". destruct σ1 as [r m]; simpl.
     iDestruct "Hσ1" as "[Hr Hm]".
     iDestruct (gen_heap_valid_inclSepM with "Hr Hmap") as %Hregs.
     have HPC' := regs_lookup_eq _ _ _ HPC.
     have ? := lookup_weaken _ _ _ _ HPC Hregs.
     iDestruct (@gen_heap_valid with "Hm Hpc_a") as %Hpc_a; auto.
-    iModIntro. iSplitR. by iPureIntro; apply normal_always_head_reducible.
+    iModIntro. iSplitR. by iPureIntro; apply normal_always_base_reducible.
     iNext. iIntros (e2 σ2 efs Hpstep).
     apply prim_step_exec_inv in Hpstep as (-> & -> & (c & -> & Hstep)).
     iSplitR; auto. eapply step_exec_inv in Hstep; eauto.
